theories/typing/int.v
@@ -22,8 +22,8 @@ Section int.
   Lemma type_int_instr z : typed_val #z int (λ post, post z).
   Proof.
     iIntros (?????) "_ _ _ $$ _ Obs". iMod persistent_time_receipt_0 as "Time".
-    iApply wp_value. iExists -[const z]. iFrame "Obs". rewrite tctx_interp_singleton
-    tctx_hasty_val'; [|done]. iExists 0%nat. iFrame "Time". by iExists z.
+    iApply wp_value. iExists -[const z]. iFrame "Obs". iSplit; [|done].
+    rewrite tctx_hasty_val'; [|done]. iExists 0%nat. iFrame "Time". by iExists z.
   Qed.
 
   Lemma type_int {As} z E L C (T: _ As) x e tr :
@@ -33,13 +33,13 @@ Section int.
   Proof. iIntros. iApply type_let; by [apply type_int_instr|solve_typing]. Qed.
 
   Lemma type_plus_instr E L p1 p2 :
-    ⊢ typed_instruction_ty E L +[p1 ◁ int; p2 ◁ int] (p1 + p2) int
+    ⊢ typed_instr_ty E L +[p1 ◁ int; p2 ◁ int] (p1 + p2) int
       (λ post '(-[z; z']), post (z + z')).
   Proof.
     iIntros (??(?&?&[])) "_ _ _ $$ (P1 & P2 &_) Obs".
     wp_apply (wp_hasty with "P1"). iIntros (? d) "Time". iIntros ((z&->&[=->])).
     wp_apply (wp_hasty with "P2"). iIntros (??) "_". iIntros ((z'&->&[=->])).
-    wp_op. iExists -[const (z + z')]. iFrame "Obs". rewrite tctx_interp_singleton
+    wp_op. iExists -[const (z + z')]. iFrame "Obs". rewrite right_id
     tctx_hasty_val'; [|done]. iExists d. iFrame "Time". by iExists (z + z').
   Qed.
 
@@ -54,13 +54,13 @@ Section int.
   Qed.
 
   Lemma type_minus_instr E L p1 p2 :
-    ⊢ typed_instruction_ty E L +[p1 ◁ int; p2 ◁ int] (p1 - p2) int
+    ⊢ typed_instr_ty E L +[p1 ◁ int; p2 ◁ int] (p1 - p2) int
       (λ post '(-[z; z']), post (z - z')).
   Proof.
     iIntros (??(?&?&[])) "_ _ _ $$ (P1 & P2 &_) Obs".
     wp_apply (wp_hasty with "P1"). iIntros (? d) "Time". iIntros ((z&->&[=->])).
     wp_apply (wp_hasty with "P2"). iIntros (??) "_". iIntros ((z'&->&[=->])).
-    wp_op. iExists -[const (z - z')]. iFrame "Obs". rewrite tctx_interp_singleton
+    wp_op. iExists -[const (z - z')]. iFrame "Obs". rewrite right_id
     tctx_hasty_val'; [|done]. iExists d. iFrame "Time". by iExists (z - z').
   Qed.
 
@@ -75,14 +75,14 @@ Section int.
   Qed.
 
   Lemma type_le_instr E L p1 p2 :
-    ⊢ typed_instruction_ty E L +[p1 ◁ int; p2 ◁ int] (p1 ≤ p2) bool_ty
+    ⊢ typed_instr_ty E L +[p1 ◁ int; p2 ◁ int] (p1 ≤ p2) bool_ty
       (λ post '(-[z; z']), post (bool_decide (z ≤ z'))).
   Proof.
     iIntros (??(?&?&[])) "_ _ _ $$ (P1 & P2 &_) Obs".
     wp_apply (wp_hasty with "P1"). iIntros (? d) "Time". iIntros ((z&->&[=->])).
     wp_apply (wp_hasty with "P2"). iIntros (??) "_". iIntros ((z'&->&[=->])).
     wp_op. iExists -[const (bool_decide (z <= z'))]. iFrame "Obs".
-    rewrite tctx_interp_singleton tctx_hasty_val'; [|done]. iExists d.
+    rewrite right_id tctx_hasty_val'; [|done]. iExists d.
     iFrame "Time". by iExists (bool_decide (z <= z')).
   Qed.
 
