theories/typing/uniq_bor.v
@@ -109,11 +109,7 @@ Section typing.
   Context `{!typeG Σ}.
 
   Global Instance uniq_type_contractive {A} κ : TypeContractive (@uniq_bor _ _ A κ).
-  Proof. split.
-    - apply (type_lft_morphism_add _ κ [κ] [])=> ?; [by iApply lft_equiv_refl|].
-      by rewrite elctx_interp_app elctx_interp_ty_outlives_E /elctx_interp
-        /= left_id right_id.
-    - done.
+  Proof. split; [by apply (type_lft_morphism_add_one κ)|done| |].
     - move=> */=. do 17 (f_contractive || f_equiv). by simpl in *.
     - move=> */=. do 10 (f_contractive || f_equiv). by simpl in *.
   Qed.
